pulse/share/steel/examples/pulse/dice/cbor/CBOR.Pulse.fst
@@ -67,6 +67,315 @@ val stick_weaken_hyp_l
 
 assume Fits_u64 : squash (SZ.fits_u64)
 
+module U8 = FStar.UInt8
+module U64 = FStar.UInt64
+module I16 = FStar.Int16
+
+inline_for_extraction noextract [@@noextract_to "krml"]
+let impl_compare_u8
+    (x1 x2: U8.t)
+: Tot I16.t
+= if x1 = x2
+  then 0s
+  else if x1 `U8.lt` x2
+  then -1s
+  else 1s
+
+let impl_compare_u8_correct
+    (x1 x2: U8.t)
+: Lemma
+    (I16.v (impl_compare_u8 x1 x2) == Cbor.int_compare (U8.v x1) (U8.v x2))
+    [SMTPat (impl_compare_u8 x1 x2)]
+= ()
+
+inline_for_extraction noextract [@@noextract_to "krml"]
+let impl_compare_u64
+    (x1 x2: U64.t)
+: Tot I16.t
+= if x1 = x2
+  then 0s
+  else if x1 `U64.lt` x2
+  then -1s
+  else 1s
+
+let impl_compare_u64_correct
+    (x1 x2: U64.t)
+: Lemma
+    (I16.v (impl_compare_u64 x1 x2) == Cbor.int_compare (U64.v x1) (U64.v x2))
+    [SMTPat (impl_compare_u64 x1 x2)]
+= ()
+
+
+```pulse
+fn byte_array_compare
+  (sz: SZ.t)
+  (a1: A.larray U8.t (SZ.v sz))
+  (a2: A.larray U8.t (SZ.v sz))
+  (#p1: perm)
+  (#p2: perm)
+  (#va1: Ghost.erased (Seq.seq U8.t))
+  (#va2: Ghost.erased (Seq.seq U8.t))
+requires
+    (A.pts_to a1 #p1 va1 ** A.pts_to a2 #p2 va2)
+returns res: I16.t
+ensures
+        A.pts_to a1 #p1 va1 ** A.pts_to a2 #p2 va2 **
+        pure (I16.v res == Cbor.bytes_lex_compare va1 va2)
+{
+    A.pts_to_len a1;
+    A.pts_to_len a2;
+    let mut pi = 0sz;
+    let mut pres = 0s;
+    let prf1 : squash (Ghost.reveal va1 `Seq.equal` Seq.slice va1 0 (SZ.v sz)) = ();
+    let prf2 : squash (Ghost.reveal va2 `Seq.equal` Seq.slice va2 0 (SZ.v sz)) = ();
+    while (let i = !pi; let res = !pres; ((i `SZ.lt` sz) && (res = 0s)))
+    invariant cont . exists i res .
+        A.pts_to a1 #p1 va1 ** A.pts_to a2 #p2 va2 **
+        pts_to pi i ** pts_to pres res **
+        pure (
+            SZ.v i <= SZ.v sz /\
+            Cbor.bytes_lex_compare va1 va2 == (
+                if res = 0s
+                then Cbor.bytes_lex_compare (Seq.slice va1 (SZ.v i) (SZ.v sz)) (Seq.slice va2 (SZ.v i) (SZ.v sz))
+                else I16.v res
+            ) /\
+            (cont == (SZ.v i < SZ.v sz && res = 0s))
+        )
+    {
+        let i = !pi;
+        let x1 = a1.(i);
+        let x2 = a2.(i);
+        let res = impl_compare_u8 x1 x2;
+        pi := i `SZ.add` 1sz;
+        pres := res;
+    };
+    !pres
+}
+```
+
+inline_for_extraction noextract [@@noextract_to "krml"]
+let i16_neq_0 (x: I16.t) : Tot bool = x <> 0s // FIXME: WHY WHY WHY?
+
+```pulse
+fn rec cbor_compare
+  (a1: cbor)
+  (a2: cbor)
+  (#p1: perm)
+  (#p2: perm)
+  (#v1: Ghost.erased Cbor.raw_data_item)
+  (#v2: Ghost.erased Cbor.raw_data_item)
+requires
+    (raw_data_item_match p1 a1 v1 ** raw_data_item_match p2 a2 v2)
+returns res: I16.t
+ensures
+    (raw_data_item_match p1 a1 v1 ** raw_data_item_match p2 a2 v2 ** pure (
+      ((I16.v res <: int) == Cbor.cbor_compare v1 v2)
+    ))
+{
+    let test = cbor_compare_aux a1 a2;
+    if (test = -1s || test = 0s || test = 1s) {
+        test
+    } else {
+        let ty1 = cbor_get_major_type a1;
+        let ty2 = cbor_get_major_type a2;
+        let c = impl_compare_u8 ty1 ty2;
+        if (i16_neq_0 c)
+        {
+            c
+        } else if (ty1 = major_type_uint64 || ty1 = major_type_neg_int64) {
+            let i1 = destr_cbor_int64 a1;
+            let i2 = destr_cbor_int64 a2;
+            (impl_compare_u64 i1.cbor_int_value i2.cbor_int_value)
+        } else if (ty1 = major_type_simple_value) {
+            let i1 = destr_cbor_simple_value a1;
+            let i2 = destr_cbor_simple_value a2;
+            (impl_compare_u8 i1 i2)
+        } else if (ty1 = major_type_byte_string || ty1 = major_type_text_string) {
+            let s1 = destr_cbor_string a1;
+            let s2 = destr_cbor_string a2;
+            let c = impl_compare_u64 s1.cbor_string_length s2.cbor_string_length;
+            if (i16_neq_0 c) {
+                elim_stick0 ();
+                elim_stick0 ();
+                c
+            } else {
+                A.pts_to_len s1.cbor_string_payload;
+                A.pts_to_len s2.cbor_string_payload;
+                let test = byte_array_compare (SZ.uint64_to_sizet s1.cbor_string_length) s1.cbor_string_payload s2.cbor_string_payload;
+                elim_stick0 ();
+                elim_stick0 ();
+                test
+            }
+        } else if (ty1 = major_type_array) {
+            let len1 = cbor_array_length a1;
+            let len2 = cbor_array_length a2;
+            let c = impl_compare_u64 len1 len2;
+            if (i16_neq_0 c) {
+                c
+            } else {
+                let i10 = cbor_array_iterator_init a1;
+                let i20 = cbor_array_iterator_init a2;
+                let done0 = cbor_array_iterator_is_done i10;
+                let mut pi1 = i10;
+                let mut pi2 = i20;
+                let mut pdone = done0;
+                let mut pres = 0s;
+                while (
+                    let done = !pdone;
+                    let res = !pres;
+                    (res = 0s && not done)
+                )
+                invariant cont . exists i1 i2 done res l1 l2 .
+                    pts_to pi1 i1 ** pts_to pi2 i2 ** pts_to pdone done ** pts_to pres res **
+                    cbor_array_iterator_match p1 i1 l1 **
+                    cbor_array_iterator_match p2 i2 l2 **
+                    `@(cbor_array_iterator_match p1 i1 l1 @==> raw_data_item_match p1 a1 v1) **
+                    `@(cbor_array_iterator_match p2 i2 l2 @==> raw_data_item_match p2 a2 v2) **
+                    pure (
+                        List.Tot.length l1 == List.Tot.length l2 /\
+                        Cbor.cbor_compare v1 v2 == (if res = 0s then Cbor.cbor_compare_array l1 l2 else I16.v res) /\
+                        (res == 0s ==> done == Nil? l1) /\
+                        cont == (Cons? l1 && res = 0s)
+                    )
+                {
+                    let x1 = cbor_array_iterator_next pi1;
+                    with v1' . assert (raw_data_item_match p1 x1 v1');
+                    let x2 = cbor_array_iterator_next pi2;
+                    with v2' . assert (raw_data_item_match p2 x2 v2');
+                    let res = cbor_compare x1 x2;
+                    with gi1' l1' . assert (pts_to pi1 gi1' ** cbor_array_iterator_match p1 gi1' l1');
+                    with gi2' l2' . assert (pts_to pi2 gi2' ** cbor_array_iterator_match p2 gi2' l2');
+                    stick_consume_l ()
+                        #(raw_data_item_match p1 x1 v1')
+                        #(cbor_array_iterator_match p1 gi1' l1');
+                    stick_consume_l ()
+                        #(raw_data_item_match p2 x2 v2')
+                        #(cbor_array_iterator_match p2 gi2' l2');
+                    stick_trans ()
+                        #(cbor_array_iterator_match p1 gi1' l1');
+                    stick_trans ()
+                        #(cbor_array_iterator_match p2 gi2' l2');
+                    if (res = 0s) {
+                        let i1 = !pi1;
+                        rewrite each gi1' as i1;
+                        let done = cbor_array_iterator_is_done i1;
+                        pdone := done
+                    } else {
+                        pres := res
+                    }
+                };
+                elim_stick0 ();
+                elim_stick0 ();
+                !pres
+            }
+        } else if (ty1 = major_type_tagged) {
+            let tg1 = destr_cbor_tagged a1;
+            let tg2 = destr_cbor_tagged a2;
+            let c = impl_compare_u64 tg1.cbor_tagged_tag tg2.cbor_tagged_tag;
+            if (i16_neq_0 c) {
+                elim_stick0 ();
+                elim_stick0 ();
+                c
+            } else {
+                with v1' . assert (raw_data_item_match p1 tg1.cbor_tagged_payload v1');
+                with v2' . assert (raw_data_item_match p2 tg2.cbor_tagged_payload v2');
+                let test = cbor_compare tg1.cbor_tagged_payload tg2.cbor_tagged_payload;
+                elim_stick0 ();
+                elim_stick0 ();
+                test
+            }
+        } else if (ty1 = major_type_map) {
+            let len1 = cbor_map_length a1;
+            let len2 = cbor_map_length a2;
+            let c = impl_compare_u64 len1 len2;
+            if (i16_neq_0 c) {
+                c
+            } else {
+                let i10 = cbor_map_iterator_init a1;
+                let i20 = cbor_map_iterator_init a2;
+                let done0 = cbor_map_iterator_is_done i10;
+                let mut pi1 = i10;
+                let mut pi2 = i20;
+                let mut pdone = done0;
+                let mut pres = 0s;
+                while (
+                    let done = !pdone;
+                    let res = !pres;
+                    (res = 0s && not done)
+                )
+                invariant cont . exists i1 i2 done res l1 l2 .
+                    pts_to pi1 i1 ** pts_to pi2 i2 ** pts_to pdone done ** pts_to pres res **
+                    cbor_map_iterator_match p1 i1 l1 **
+                    cbor_map_iterator_match p2 i2 l2 **
+                    `@(cbor_map_iterator_match p1 i1 l1 @==> raw_data_item_match p1 a1 v1) **
+                    `@(cbor_map_iterator_match p2 i2 l2 @==> raw_data_item_match p2 a2 v2) **
+                    pure (
+                        List.Tot.length l1 == List.Tot.length l2 /\
+                        (Cbor.cbor_compare v1 v2 == (if res = 0s then Cbor.cbor_compare_map l1 l2 else I16.v res)) /\
+                        (res == 0s ==> done == Nil? l1) /\
+                        cont == (Cons? l1 && res = 0s)
+                    )
+                {
+                    let x1 = cbor_map_iterator_next pi1;
+                    with v1' . assert (raw_data_item_map_entry_match p1 x1 v1');
+                    with gi1' l1' . assert (pts_to pi1 gi1' ** cbor_map_iterator_match p1 gi1' l1');
+                    stick_trans ()
+                        #(raw_data_item_map_entry_match p1 x1 v1' ** cbor_map_iterator_match p1 gi1' l1');
+                    let x2 = cbor_map_iterator_next pi2;
+                    with v2' . assert (raw_data_item_map_entry_match p2 x2 v2');
+                    with gi2' l2' . assert (pts_to pi2 gi2' ** cbor_map_iterator_match p2 gi2' l2');
+                    stick_trans ()
+                        #(raw_data_item_map_entry_match p2 x2 v2' ** cbor_map_iterator_match p2 gi2' l2');
+                    unfold (raw_data_item_map_entry_match p1 x1 v1');
+                    unfold (raw_data_item_map_entry_match p2 x2 v2');
+                    let test = cbor_compare (cbor_map_entry_key x1) (cbor_map_entry_key x2);
+                    if (test = 0s) ensures exists res done . // FIXME: HOW HOW HOW can I frame some things out?
+                        pts_to pi1 gi1' ** pts_to pi2 gi2' ** pts_to pdone done **
+                        raw_data_item_match p1 (cbor_map_entry_key x1) (fstp v1') **
+                        raw_data_item_match p2 (cbor_map_entry_key x2) (fstp v2') **
+                        raw_data_item_match p1 (cbor_map_entry_value x1) (sndp v1') **
+                        raw_data_item_match p2 (cbor_map_entry_value x2) (sndp v2') **
+                        cbor_map_iterator_match p1 gi1' l1' **
+                        cbor_map_iterator_match p2 gi2' l2' **
+                        `@((raw_data_item_map_entry_match p1 x1 v1' ** cbor_map_iterator_match p1 gi1' l1') @==> raw_data_item_match p1 a1 v1) **
+                        `@((raw_data_item_map_entry_match p2 x2 v2' ** cbor_map_iterator_match p2 gi2' l2') @==> raw_data_item_match p2 a2 v2) **
+                        pts_to pres res ** pure ((I16.v res <: int) == (if Cbor.cbor_compare (fstp v1') (fstp v2') <> 0 then Cbor.cbor_compare (fstp v1') (fstp v2') else Cbor.cbor_compare (sndp v1') (sndp v2')))
+                    {
+                        let test = cbor_compare (cbor_map_entry_value x1) (cbor_map_entry_value x2);
+                        pres := test;
+                    } else {
+                        pres := test;
+                    };
+                    fold (raw_data_item_map_entry_match p1 x1 v1');
+                    fold (raw_data_item_map_entry_match p2 x2 v2');
+                    stick_consume_l ()
+                        #(raw_data_item_map_entry_match p1 x1 v1')
+                        #(cbor_map_iterator_match p1 gi1' l1');
+                    stick_consume_l ()
+                        #(raw_data_item_map_entry_match p2 x2 v2')
+                        #(cbor_map_iterator_match p2 gi2' l2');
+                    let res = !pres;
+                    if (res = 0s) {
+                        let i1 = !pi1;
+                        rewrite each gi1' as i1;
+                        let done = cbor_map_iterator_is_done i1;
+                        pdone := done
+                    }
+                };
+                elim_stick0 ();
+                elim_stick0 ();
+                !pres
+            }
+        } else {
+            // unreachable
+            let unused : squash False = ();
+            2s
+        }
+    }
+}
+
+```
+
 ```pulse
 fn rec cbor_is_equal
   (a1: cbor)
@@ -83,212 +392,10 @@ ensures
       (res == true <==> v1 == v2)
     ))
 {
-    let test = cbor_is_equal_aux a1 a2;
-    match test {
-        CborEqual ->
-        {
-            true
-        }
-        CborNotEqual ->
-        {
-            false
-        }
-        _ ->
-        {
-            let ty1 = cbor_get_major_type a1;
-            let ty2 = cbor_get_major_type a2;
-            if (ty1 <> ty2)
-            {
-                false
-            } else if (ty1 = major_type_uint64 || ty1 = major_type_neg_int64) {
-                let i1 = destr_cbor_int64 a1;
-                let i2 = destr_cbor_int64 a2;
-                (i1.cbor_int_value = i2.cbor_int_value)
-            } else if (ty1 = major_type_simple_value) {
-                let i1 = destr_cbor_simple_value a1;
-                let i2 = destr_cbor_simple_value a2;
-                (i1 = i2)
-            } else if (ty1 = major_type_byte_string || ty1 = major_type_text_string) {
-                let s1 = destr_cbor_string a1;
-                let s2 = destr_cbor_string a2;
-                if (s1.cbor_string_length <> s2.cbor_string_length) {
-                    elim_stick0 ();
-                    elim_stick0 ();
-                    false
-                } else {
-                    A.pts_to_len s1.cbor_string_payload;
-                    A.pts_to_len s2.cbor_string_payload;
-                    let test = A.compare (SZ.uint64_to_sizet s1.cbor_string_length) s1.cbor_string_payload s2.cbor_string_payload;
-                    elim_stick0 ();
-                    elim_stick0 ();
-                    test
-                }
-            } else if (ty1 = major_type_array) {
-                let len1 = cbor_array_length a1;
-                let len2 = cbor_array_length a2;
-                if (len1 <> len2) {
-                    false
-                } else {
-                    let i10 = cbor_array_iterator_init a1;
-                    let i20 = cbor_array_iterator_init a2;
-                    let done0 = cbor_array_iterator_is_done i10;
-                    let mut pi1 = i10;
-                    let mut pi2 = i20;
-                    let mut pdone = done0;
-                    let mut pres = true;
-                    while (
-                        let done = !pdone;
-                        let res = !pres;
-                        (res && not done)
-                    )
-                    invariant cont . exists i1 i2 done res l1 l2 .
-                        pts_to pi1 i1 ** pts_to pi2 i2 ** pts_to pdone done ** pts_to pres res **
-                        cbor_array_iterator_match p1 i1 l1 **
-                        cbor_array_iterator_match p2 i2 l2 **
-                        `@(cbor_array_iterator_match p1 i1 l1 @==> raw_data_item_match p1 a1 v1) **
-                        `@(cbor_array_iterator_match p2 i2 l2 @==> raw_data_item_match p2 a2 v2) **
-                        pure (
-                            List.Tot.length l1 == List.Tot.length l2 /\
-                            (Ghost.reveal (v1 == v2) <==> (res == true /\ l1 == l2)) /\
-                            (res == true ==> done == Nil? l1) /\
-                            cont == (Cons? l1 && res)
-                        )
-                    {
-                        let x1 = cbor_array_iterator_next pi1;
-                        with v1' . assert (raw_data_item_match p1 x1 v1');
-                        let x2 = cbor_array_iterator_next pi2;
-                        with v2' . assert (raw_data_item_match p2 x2 v2');
-                        let test = cbor_is_equal x1 x2;
-                        with gi1' l1' . assert (pts_to pi1 gi1' ** cbor_array_iterator_match p1 gi1' l1');
-                        with gi2' l2' . assert (pts_to pi2 gi2' ** cbor_array_iterator_match p2 gi2' l2');
-                        stick_consume_l ()
-                            #(raw_data_item_match p1 x1 v1')
-                            #(cbor_array_iterator_match p1 gi1' l1');
-                        stick_consume_l ()
-                            #(raw_data_item_match p2 x2 v2')
-                            #(cbor_array_iterator_match p2 gi2' l2');
-                        stick_trans ()
-                            #(cbor_array_iterator_match p1 gi1' l1');
-                        stick_trans ()
-                            #(cbor_array_iterator_match p2 gi2' l2');
-                        if (test) {
-                            let i1 = !pi1;
-                            rewrite each gi1' as i1;
-                            let done = cbor_array_iterator_is_done i1;
-                            pdone := done
-                        } else {
-                            pres := false
-                        }
-                    };
-                    elim_stick0 ();
-                    elim_stick0 ();
-                    !pres
-                }
-            } else if (ty1 = major_type_tagged) {
-                let tg1 = destr_cbor_tagged a1;
-                let tg2 = destr_cbor_tagged a2;
-                if (tg1.cbor_tagged_tag <> tg2.cbor_tagged_tag) {
-                    elim_stick0 ();
-                    elim_stick0 ();
-                    false
-                } else {
-                    with v1' . assert (raw_data_item_match p1 tg1.cbor_tagged_payload v1');
-                    with v2' . assert (raw_data_item_match p2 tg2.cbor_tagged_payload v2');
-                    let test = cbor_is_equal tg1.cbor_tagged_payload tg2.cbor_tagged_payload;
-                    elim_stick0 ();
-                    elim_stick0 ();
-                    test
-                }
-            } else if (ty1 = major_type_map) {
-                let len1 = cbor_map_length a1;
-                let len2 = cbor_map_length a2;
-                if (len1 <> len2) {
-                    false
-                } else {
-                    let i10 = cbor_map_iterator_init a1;
-                    let i20 = cbor_map_iterator_init a2;
-                    let done0 = cbor_map_iterator_is_done i10;
-                    let mut pi1 = i10;
-                    let mut pi2 = i20;
-                    let mut pdone = done0;
-                    let mut pres = true;
-                    while (
-                        let done = !pdone;
-                        let res = !pres;
-                        (res && not done)
-                    )
-                    invariant cont . exists i1 i2 done res l1 l2 .
-                        pts_to pi1 i1 ** pts_to pi2 i2 ** pts_to pdone done ** pts_to pres res **
-                        cbor_map_iterator_match p1 i1 l1 **
-                        cbor_map_iterator_match p2 i2 l2 **
-                        `@(cbor_map_iterator_match p1 i1 l1 @==> raw_data_item_match p1 a1 v1) **
-                        `@(cbor_map_iterator_match p2 i2 l2 @==> raw_data_item_match p2 a2 v2) **
-                        pure (
-                            List.Tot.length l1 == List.Tot.length l2 /\
-                            (Ghost.reveal (v1 == v2) <==> (res == true /\ l1 == l2)) /\
-                            (res == true ==> done == Nil? l1) /\
-                            cont == (Cons? l1 && res)
-                        )
-                    {
-                        let x1 = cbor_map_iterator_next pi1;
-                        with v1' . assert (raw_data_item_map_entry_match p1 x1 v1');
-                        with gi1' l1' . assert (pts_to pi1 gi1' ** cbor_map_iterator_match p1 gi1' l1');
-                        stick_trans ()
-                            #(raw_data_item_map_entry_match p1 x1 v1' ** cbor_map_iterator_match p1 gi1' l1');
-                        let x2 = cbor_map_iterator_next pi2;
-                        with v2' . assert (raw_data_item_map_entry_match p2 x2 v2');
-                        with gi2' l2' . assert (pts_to pi2 gi2' ** cbor_map_iterator_match p2 gi2' l2');
-                        stick_trans ()
-                            #(raw_data_item_map_entry_match p2 x2 v2' ** cbor_map_iterator_match p2 gi2' l2');
-                        unfold (raw_data_item_map_entry_match p1 x1 v1');
-                        unfold (raw_data_item_map_entry_match p2 x2 v2');
-                        let test = cbor_is_equal (cbor_map_entry_key x1) (cbor_map_entry_key x2);
-                        if test ensures exists res done . // FIXME: HOW HOW HOW can I frame some things out?
-                            pts_to pi1 gi1' ** pts_to pi2 gi2' ** pts_to pdone done **
-                            raw_data_item_match p1 (cbor_map_entry_key x1) (fstp v1') **
-                            raw_data_item_match p2 (cbor_map_entry_key x2) (fstp v2') **
-                            raw_data_item_match p1 (cbor_map_entry_value x1) (sndp v1') **
-                            raw_data_item_match p2 (cbor_map_entry_value x2) (sndp v2') **
-                            cbor_map_iterator_match p1 gi1' l1' **
-                            cbor_map_iterator_match p2 gi2' l2' **
-                            `@((raw_data_item_map_entry_match p1 x1 v1' ** cbor_map_iterator_match p1 gi1' l1') @==> raw_data_item_match p1 a1 v1) **
-                            `@((raw_data_item_map_entry_match p2 x2 v2' ** cbor_map_iterator_match p2 gi2' l2') @==> raw_data_item_match p2 a2 v2) **
-                            pts_to pres res ** pure (res == true <==> v1' == v2')
-                        {
-                            let test = cbor_is_equal (cbor_map_entry_value x1) (cbor_map_entry_value x2);
-                            pres := test;
-                        } else {
-                            pres := false;
-                        };
-                        fold (raw_data_item_map_entry_match p1 x1 v1');
-                        fold (raw_data_item_map_entry_match p2 x2 v2');
-                        stick_consume_l ()
-                            #(raw_data_item_map_entry_match p1 x1 v1')
-                            #(cbor_map_iterator_match p1 gi1' l1');
-                        stick_consume_l ()
-                            #(raw_data_item_map_entry_match p2 x2 v2')
-                            #(cbor_map_iterator_match p2 gi2' l2');
-                        let res = !pres;
-                        if (res) {
-                            let i1 = !pi1;
-                            rewrite each gi1' as i1;
-                            let done = cbor_map_iterator_is_done i1;
-                            pdone := done
-                        }
-                    };
-                    elim_stick0 ();
-                    elim_stick0 ();
-                    !pres
-                }
-            } else {
-                // unreachable
-                let unused : squash False = ();
-                false
-            }
-        }
-    }
+    Cbor.cbor_compare_equal v1 v2;
+    let test = cbor_compare a1 a2;
+    (test = 0s)
 }
-
 ```
 
 noeq
